add opt examples

theories/opt/ex2_2.v
@@ -2,8 +2,10 @@ From stbor.sim Require Import local invariant one_step.
 
 Set Default Proof Using "Type".
 
+(* Assuming x : & i32 *)
 Definition ex2_2 : function :=
-  fun: ["x"],
+  fun: ["i"],
+    let: "x" := new_place (& int) &"i" in
     Retag "x"  FnEntry ;;
     let: "v" := Copy *{int} "x" in
     Call #[ScFnPtr "f"] ["x"] ;;
@@ -11,8 +13,21 @@ Definition ex2_2 : function :=
     .
 
 Definition ex2_2_opt : function :=
-  fun: ["x"],
+  fun: ["i"],
+    let: "x" := new_place (& int) &"i" in
     Retag "x"  FnEntry ;;
     Call #[ScFnPtr "f"] ["x"] ;;
     Copy *{int} "x"
     .
+
+
+Lemma ex2_2_sim_fun fs ft : ⊨{fs,ft} ex2_2 ≥ᶠ ex2_2_opt.
+Proof.
+  intros r es et els elt σs σt FAs FAt FREL SUBSTs SUBSTt.
+  destruct els as [|efs []]; [done| |done].  simpl in SUBSTs.
+  destruct elt as [|eft []]; [done| |done].  simpl in SUBSTt. simplify_eq.
+
+  (* InitCall *)
+  exists 10%nat.
+  apply sim_body_init_call. simpl.
+Abort.
