theories/opt/ex1.v
@@ -1,0 +1,29 @@
+From stbor.sim Require Import local invariant one_step.
+
+Set Default Proof Using "Type".
+
+(* Assuming x : &mut i32 *)
+Definition ex1 : expr :=
+  let: "x" := new_place (&mut int) &"i" in
+  Retag "x" Default ;;
+  Call #[ScFnPtr "f"] [] ;;
+  *{int} "x" <- #[42] ;;
+  Call #[ScFnPtr "g"] [] ;;
+  Copy *{int} "x"
+  .
+
+Definition ex1_opt : expr :=
+  let: "x" := new_place (&mut int) &"i" in
+  Retag "x" Default ;;
+  Call #[ScFnPtr "f"] [] ;;
+  *{int} "x" <- #[42] ;;
+  let: "v" := Copy *{int} "x" in
+  Call #[ScFnPtr "g"] [] ;;
+  "v"
+  .
+
+Lemma ex1_sim_body fs ft r n σs σt :
+  (* TODO: what's in r? *)
+  r ⊨{n, fs,ft} (ex1, σs) ≥ (ex1_opt, σt) : (λ r' _ vs' σs' vt' σt', vrel_expr r' vs' vt').
+Proof.
+Abort.
