theories/opt/ex1_2.v
@@ -2,36 +2,40 @@ From stbor.sim Require Import local invariant one_step.
 
 Set Default Proof Using "Type".
 
+(* Assuming x : &mut i32 *)
 Definition ex1_2 : function :=
-  fun: ["x"],
+  fun: ["i"],
+  let: "x" := new_place (&mut int) &"i" in
   Retag "x"  FnEntry ;;
-  *{int} (Copy1 "x") <- #[42] ;;
+  *{int} "x" <- #[42] ;;
   Call #[ScFnPtr "f"] [] ;;
-  *{int} (Copy1 "x") <- #[13]
+  *{int} "x" <- #[13]
   .
 
 Definition ex1_2_opt_1 : function :=
-  fun: ["x"],
+  fun: ["i"],
+  let: "x" := new_place (&mut int) &"i" in
   Retag "x"  FnEntry ;;
   Call #[ScFnPtr "f"] [] ;;
-  *{int} (Copy1 "x") <- #[42] ;;
-  *{int} (Copy1 "x") <- #[13]
+  *{int} "x" <- #[42] ;;
+  *{int} "x" <- #[13]
   .
 
 Definition ex1_2_opt_2 : function :=
-  fun: ["x"],
+  fun: ["i"],
+  let: "x" := new_place (&mut int) &"i" in
   Retag "x"  FnEntry ;;
   Call #[ScFnPtr "f"] [] ;;
-  *{int} (Copy1 "x") <- #[13]
+  *{int} "x" <- #[13]
   .
 
 Lemma ex1_2_sim_fun fs ft : ⊨{fs,ft} ex1_2 ≥ᶠ ex1_2_opt_1.
 Proof.
-  intros [r1 r2] es et els elt σs σt FAs FAt FREL SUBSTs SUBSTt.
+  intros r es et els elt σs σt FAs FAt FREL SUBSTs SUBSTt.
   destruct els as [|efs []]; [done| |done].  simpl in SUBSTs.
   destruct elt as [|eft []]; [done| |done].  simpl in SUBSTt. simplify_eq.
 
   (* InitCall *)
-  exists 1%nat.
-  apply sim_body_init_call. rewrite pair_op.
+  exists 10%nat.
+  apply sim_body_init_call. simpl.
 Abort.
